examples/crypto/dh_hye/HyE.DH.fst
@@ -8,7 +8,6 @@ open FStar.HyperHeap
 open FStar.HyperStack
 open FStar.Monotonic.RRef
 open FStar.Seq
-open FStar.SeqProperties
 open FStar.Monotonic.Seq
 open FStar.List.Tot
 
@@ -19,18 +18,20 @@ open HyE.Indexing
 open HyE.PlainDH
 open HyE.Flags
 
+module HH = FStar.HyperHeap
+module MM = MonotoneMap
 
 assume val dh_share_size : nat
 assume val dh_exponent_size : nat
 type dh_share = lbytes dh_share_size
 abstract type dh_exponent = lbytes dh_exponent_size
 
-assume val dh_gen_key: unit -> St (dh_share*dh_exponent)
+assume val dh_gen_key: unit -> Tot (dh_share*dh_exponent)
 
 type keysize = aeadKeySize AES_128_GCM
 type aes_key = lbytes keysize (* = b:bytes{B.length b = keysize} *)
 
-type log_t (i:id) (r:rid) = m_rref r (seq (entry:(PlainDH.key*dh_share){fst (AE.get_index (fst entry)) = i})) grows
+type log_t (i:id) (r:rid) = m_rref r (seq (entry:(PlainDH.key*dh_share){ae_fixed (PlainDH.get_index (fst entry))})) grows
 
 noeq type dh_pkey = 
   | DH_pkey:  #pk_i:id -> #region:rid ->rawpk:dh_share -> log:log_t pk_i region -> dh_pkey
@@ -42,19 +43,26 @@ noeq abstract type dh_skey =
 val get_index: dh_skey -> Tot(id)
 let get_index k = k.sk_i
 
-val keygen: #i:id -> (parent:rid) -> ST (dh_pair:(k:dh_pkey{k.pk_i=i}) * (k:dh_skey{k.sk_i=i}))
-  (requires (fun h -> True))
-  (ensures (fun h0 k h1 -> True
+val keygen: #i:id -> (parent:rid{disjoint id_honesty_table_region parent}) -> ST (dh_pair:(k:dh_pkey{k.pk_i=i}) * (k:dh_skey{k.sk_i=i}))
+  (requires (fun h -> fresh i h /\ MM.fresh id_honesty_table i h))
+  (ensures (fun h0 k h1 ->
+    let (s:Set.set (HH.rid)) = Set.union (Set.singleton parent) (Set.singleton id_freshness_table_region) in
+    modifies s h0 h1
+    /\ MM.fresh id_honesty_table i h1
+    /\ unfresh i
 //  let (pk,sk) = k in
 //  safe_key_gen parent pk h0 h1
   ))
 let keygen #i parent =
+  make_unfresh i;
   let region = new_region parent in
   let log = alloc_mref_seq region createEmpty in
   let dh_share,dh_exponent = dh_gen_key() in
   let dh_pk = DH_pkey #i #region dh_share log in
   let dh_sk = DH_skey #i dh_exponent dh_pk in
+  let h1 = ST.get() in
   dh_pk,dh_sk
+
 
 (**
    This function takes a dh_share to the power of a dh_exponent.
@@ -73,14 +81,16 @@ type safe_log_append pk entry h0 h1 =
    share and exponent are honest.
 *)
 val prf_odh_snd: sk:dh_skey -> pk:dh_pkey -> ST (PlainDH.key)
-  ( requires (fun _ -> True))
-  ( ensures (fun _ k _ -> HyE.AE.get_index k = (pk.pk_i, sk.sk_i)
+  ( requires (fun _ -> ae_fixed (generate_ae_id sk.sk_i pk.pk_i)))
+  ( ensures (fun _ k _ -> 
+    HyE.AE.get_index k = generate_ae_id pk.pk_i sk.sk_i
   ))
 let prf_odh_snd dh_snd_sk dh_rcv_pk =
   let pk_id = dh_rcv_pk.pk_i in
   let sk_id = dh_snd_sk.sk_i in
-  let i = pk_id, sk_id in
-  if ae_honest i && prf_odh then
+  let i = generate_ae_id pk_id sk_id in
+  let ae_honest_i = ae_honestST i in
+  if ae_honest_i && prf_odh then
     let k' = PlainDH.keygen i dh_rcv_pk.region in
     write_at_end dh_rcv_pk.log (k',dh_snd_sk.pk.rawpk);
     k'
@@ -94,19 +104,29 @@ let equal_share dh_sh entry =
   snd entry = dh_sh
 
 
-val prf_odh_rcv: #(sk_id:id) -> dh_sh:dh_share -> dh_sk:dh_skey -> St (k:PlainDH.key)//{fst (AE.get_index k) = sk_id})
+val prf_odh_rcv: #(sk_id:id{fixed sk_id}) -> dh_sh:dh_share -> dh_sk:dh_skey -> ST (k:PlainDH.key)//{fst (AE.get_index k) = sk_id})
+  (requires (fun h0 -> True))
+  (ensures (fun h0 k h1 ->
+    ae_fixed (PlainDH.get_index k)
+  ))
 let prf_odh_rcv #sk_id dh_sh dh_rcv_sk =
-  if honest sk_id && prf_odh then
+  let honest_sk_id = honestST sk_id in
+  if honest_sk_id && prf_odh then
     let log = m_read dh_rcv_sk.pk.log in
     let entry = seq_find (equal_share dh_sh) log in
     match entry with
     | Some (k',_) -> k'
     | None -> 
-      let i = sk_id,dishonestId() in
+      let dis_id = generate_fresh_id() in
+      make_unfresh dis_id;
+      make_dishonest dis_id;
+      let i = generate_ae_id sk_id dis_id in
       let raw_k = dh_exponentiate dh_sh dh_rcv_sk.rawsk in
       PlainDH.coerce_key i dh_rcv_sk.pk.region raw_k
   else
-    let dis_id = dishonestId() in
-    let i =  sk_id,dis_id in
+    let dis_id = generate_fresh_id() in
+    make_unfresh dis_id;
+    make_dishonest dis_id;
+    let i = generate_ae_id sk_id dis_id in
     let raw_k = dh_exponentiate dh_sh dh_rcv_sk.rawsk in
     PlainDH.coerce_key i dh_rcv_sk.pk.region raw_k
