examples/crypto/dh_hye/HyE.PlainHPKE.fst
@@ -21,15 +21,13 @@ let get_index p =
   p.i
 
 (* two pure functions, never called when ideal *)
-val repr: p:protected_hpke_plain{not hpke_ind_cca || not (ae_honest p.i)} -> Tot hpke_plain
+val repr: p:protected_hpke_plain{not hpke_ind_cca \/ (ae_dishonest p.i) } -> Tot hpke_plain
 let repr p = p.b
 
 // Change this if we want to use signcryption with hpke_int-ctxt
-val coerce: #i:ae_id -> p:hpke_plain{not hpke_ind_cca || not (ae_honest i)} -> Tot (prot:protected_hpke_plain{i=prot.i})
+val coerce: #i:ae_id -> p:hpke_plain{not hpke_ind_cca \/ (ae_dishonest i)} -> Tot (prot:protected_hpke_plain{i=prot.i})
 let coerce #i p = 
   Prot_hpke_p #i p  
 
 val length: #i:ae_id -> protected_hpke_plain -> Tot nat
 let length #i p = length p.b
-
-// Create coece_keyshare function
